Full pipeline working again

src/Assembly/PseudoConversion.v
@@ -1,185 +1,202 @@
-
 Require Export Language Conversion QhasmEvalCommon QhasmUtil.
 Require Export Pseudo AlmostQhasm State.
-Require Export Bedrock.Word NArith NPeano Euclid.
-Require Export List Sumbool Vector.
+Require Import Bedrock.Word NArith NPeano Euclid.
+Require Import List Sumbool Vector.
 
 Module PseudoConversion <: Conversion Pseudo AlmostQhasm.
-  Import QhasmCommon AlmostQhasm EvalUtil Util Pseudo StateCommon.
-  Import ListNotations.
+  Import AlmostQhasm EvalUtil ListState Util Pseudo ListNotations.
 
-  Definition MMap {w} := NatM.t (Mapping w).
-  Definition mempty {w} := NatM.empty (Mapping w).
+  Section Conv.
+    Variable w: nat.
+    Variable s: Width w.
 
-  Definition FMap {w} := NatM.t (AlmostProgram * (list (Mapping w))).
-  Definition fempty {w} := NatM.empty (AlmostProgram * (list (Mapping w))).
+    Definition MMap := NatM.t (Mapping w).
+    Definition mempty := NatM.empty (Mapping w).
 
-  Definition getStart {w s n m} (prog: @Pseudo w s n m) :=
-    let ns := (fix getStart' {n' m'} (p': @Pseudo w s n' m') :=
-      match p' with
-      | PVar _ _ i => [proj1_sig i]
-      | PBin _ _ p => getStart' p
-      | PDual _ _ p => getStart' p
-      | PCarry _ _ p => getStart' p
-      | PShift _ _ _ p => getStart' p
-      | PIf _ _ _ _ _ l r => (getStart' l) ++ (getStart' r)
-      | PFunExp _ p _ => getStart' p
-      | PLet _ k _ a b => (n + k) :: (getStart' a) ++ (getStart' b)
-      | PComb _ _ _ a b => (getStart' a) ++ (getStart' b)
-      | PCall _ _ _ p => getStart' p
-      | _ => []
-      end) _ _ prog in
+    Definition FMap := NatM.t (AlmostProgram * (list (Mapping w))).
+    Definition fempty := NatM.empty (AlmostProgram * (list (Mapping w))).
 
-    maxN (n :: m :: ns).
+    Definition getStart {n m} (prog: @Pseudo w s n m) :=
+      let ns := (fix getStart' {n' m'} (prog': @Pseudo w s n' m') :=
+        match prog' with
+        | PVar _ _ i => [proj1_sig i]
+        | PBin _ _ p => getStart' p
+        | PDual _ _ p => getStart' p
+        | PCarry _ _ p => getStart' p
+        | PShift _ _ _ p => getStart' p
+        | PFunExp _ p _ => getStart' p
+        | PCall _ _ _ p => getStart' p
+        | PIf _ _ _ _ _ l r => (getStart' l) ++ (getStart' r)
+        | PLet _ k _ a b => (n + k) :: (getStart' a) ++ (getStart' b)
+        | PComb _ _ _ a b => (getStart' a) ++ (getStart' b)
+        | _ => []
+        end) _ _ prog in
 
-  Definition addMap {T} (a b: NatM.t T): NatM.t T :=
-    (fix add' (m: NatM.t T) (elts: list (nat * T)%type) :=
-      match elts with
-      | [] => m
-      | (k, v) :: elts' => add' (NatM.add k v m) elts'
-      end) a (NatM.elements b).
+      (fix maxN (lst: list nat) :=
+        match lst with
+        | [] => O
+        | x :: xs => max x (maxN xs)
+        end) (n :: m :: ns).
 
-  Fixpoint convertProgram' {n m} (prog: Pseudo n m) (start: nat) (M: MMap) (F: FMap):
-      option (AlmostProgram * (list (Mapping width)) * MMap * FMap) :=
-    let rM := fun (x: nat) => regM _ (reg width_spec x) in
-    let sM := fun (x: nat) => stackM _ (stack width_spec x) in
+    Definition addMap {T} (a b: (NatM.t T)) : NatM.t T :=
+      (fix add' (m: NatM.t T) (elts: list (nat * T)%type) :=
+        match elts with
+        | [] => m
+        | (k, v) :: elts' => add' (NatM.add k v m) elts'
+        end) a (NatM.elements b).
 
-    let reg' := reg width_spec in
-    let stack' := stack width_spec in
-    let const' := const width_spec in
+    Fixpoint convertProgram' {n m} (prog: @Pseudo w s n m) (start: nat) (M: MMap) (F: FMap) :
+        option (AlmostProgram * (list (Mapping w)) * MMap * FMap) :=
 
-    let G := fun (k: nat) =>
-      match (NatM.find k M) with
-      | Some v => v
-      | _ => rM k (* TODO: more intelligent defaults *)
-      end in
+      let rM := fun (x: nat) => regM _ (reg s x) in
+      let sM := fun (x: nat) => stackM _ (stack s x) in
+      let reg' := reg s in
+      let stack' := stack s in
+      let const' := constant s in
 
-    let madd := fun (k: nat) (f: nat -> Mapping width) => NatM.add k (f k) in
-    let fadd := fun (k: nat) (f: AlmostProgram) (r: list (Mapping width)) => NatM.add k (f, r) in
+      let G := fun (k: nat) =>
+        match (NatM.find k M) with
+        | Some v => v
+        | _ => rM k (* TODO: more intelligent defaults *)
+        end in
 
-    match prog with
-    | PVar n (Some true) i => Some (ASkip, [rM i], madd i rM M, F)
-    | PVar n (Some false) i => Some (ASkip, [sM i], madd i sM M, F)
-    | PVar n None i => Some (ASkip, [G i], M, F) 
+      let madd := fun (k: nat) (f: nat -> Mapping w) =>
+        NatM.add k (f k) in
 
-    | PConst n c => Some (AAssign (AConstInt (reg' start) (const' c)),
-                         [rM start], madd start rM M, F)
+      let fadd := fun (k: nat) (f: AlmostProgram) (r: list (Mapping w)) =>
+        NatM.add k (f, r) in
 
-    | PMem n m v i => Some (AAssign (ARegMem (reg' start) (mem width_spec v) i),
-                           [rM start], madd start rM M, F)
+      match prog with
+      | PVar n (Some true) i => Some (ASkip, [rM i], madd i rM M, F)
+      | PVar n (Some false) i => Some (ASkip, [sM i], madd i sM M, F)
+      | PVar n None i => Some (ASkip, [G i], M, F) 
 
-    | PBin n o p =>
-      match (convertProgram' p start M F) with
-      | Some (p', [regM (reg _ _ a); regM (reg _ _ b)], M', F') =>
-        Some (ASeq p' (AOp (IOpReg o (reg' a) (reg' b))),
-              [rM a], madd a rM (madd b rM M'), F')
+      | PConst n c =>
+        Some (AAssign (AConstInt (reg' start) (const' c)),
+                       [rM start], madd start rM M, F)
 
-      | Some (p', [regM (reg _ _ a); constM c], M', F') =>
-        Some (ASeq p' (AOp (IOpConst o (reg' a) c)),
-              [rM a], madd a rM M', F')
+      | PMem n m v i =>
+        Some (AAssign (ARegMem (reg' start) (mem s v) i),
+                       [rM start], madd start rM M, F)
 
-      | Some (p', [regM (reg _ _ a); memM _ b i], M', F') =>
-        Some (ASeq p' (AOp (IOpMem o (reg' a) b i)),
-              [rM a], madd a rM M', F')
+      | PBin n o p =>
+        match (convertProgram' p start M F) with
+        | Some (p', [regM (reg _ _ a); regM (reg _ _ b)], M', F') =>
+            Some (ASeq p' (AOp (IOpReg o (reg' a) (reg' b))),
+                [rM a], madd a rM (madd b rM M'), F')
 
-      | Some (p', [regM (reg _ _ a); stackM (stack _ _ b)], M', F') =>
-        Some (ASeq p' (AOp (IOpStack o (reg' a) (stack' b))),
-              [rM a], madd a rM (madd b sM M'), F')
+        | Some (p', [regM (reg _ _ a); constM c], M', F') =>
+            Some (ASeq p' (AOp (IOpConst o (reg' a) c)),
+                [rM a], madd a rM M', F')
 
-      | _ => None
-      end
+        | Some (p', [regM (reg _ _ a); memM _ b i], M', F') =>
+            Some (ASeq p' (AOp (IOpMem o (reg' a) b i)),
+                [rM a], madd a rM M', F')
 
-    | PCarry n o p =>
-      match (convertProgram' p start M F) with
-      | Some (p', [regM (reg _ _ a); regM (reg _ _ b)], M', F') =>
-        Some (ASeq p' (AOp (COp o (reg' a) (reg' b))),
-              [rM a], madd a rM (madd b rM M'), F')
+        | Some (p', [regM (reg _ _ a); stackM (stack _ _ b)], M', F') =>
+            Some (ASeq p' (AOp (IOpStack o (reg' a) (stack' b))),
+                [rM a], madd a rM (madd b sM M'), F')
 
-      | _ => None
-      end
-
-    | PDual n o p =>
-      match (convertProgram' p (S start) M F) with
-      | Some (p', [regM (reg _ _ a); regM (reg _ _ b)], M', F') =>
-        Some (ASeq p' (AOp (DOp o (reg' a) (reg' b) (Some (reg' start)))),
-              [rM a; rM start], madd a rM (madd b rM (madd start rM M')), F')
-
-      | _ => None
-      end
-
-    | PShift n o x p =>
-      match (convertProgram' p start M F) with
-      | Some (p', [regM (reg _ _ a)], M', F') =>
-        Some (ASeq p' (AOp (ROp o (reg' a) x)),
-              [rM a], madd a rM M', F')
-
-      | _ => None
-      end
-
-    | PLet n k m f g =>
-      match (convertProgram' f start M F) with
-      | None => None
-      | Some (fp, fm, M', F') =>
-        match (convertProgram' g (start + (length fm)) M' F') with
-        | None => None
-        | Some (gp, gm, M'', F'') => Some (ASeq fp gp, gm, M'', F'')
+        | _ => None
         end
-      end
 
-    | PComb n a b f g => 
-      match (convertProgram' f start M F) with
-      | None => None
-      | Some (fp, fm, M', F') =>
-        match (convertProgram' g (start + (length fm)) M' F') with
-        | None => None
-        | Some (gp, gm, M'', F'') => Some (ASeq fp gp, fm ++ gm, M'', F'')
+      | PCarry n o p =>
+        match (convertProgram' p start M F) with
+        | Some (p', [regM (reg _ _ a); regM (reg _ _ b)], M', F') =>
+            Some (ASeq p' (AOp (COp o (reg' a) (reg' b))),
+                [rM a], madd a rM (madd b rM M'), F')
+
+        | _ => None
         end
-      end
 
-    | PIf n m o i0 i1 l r => 
-      match (convertProgram' l start M F) with
-      | None => None
-      | Some (lp, lr, lM, lF) =>
+      | PDual n o p =>
+        match (convertProgram' p (S start) M F) with
+        | Some (p', [regM (reg _ _ a); regM (reg _ _ b)], M', F') =>
+            Some (ASeq p' (AOp (DOp o (reg' a) (reg' b) (Some (reg' start)))),
+                [rM a; rM start], madd a rM (madd b rM (madd start rM M')), F')
 
-        match (convertProgram' r start lM lF) with
+        | _ => None
+        end
+
+      | PShift n o x p =>
+        match (convertProgram' p start M F) with
+        | Some (p', [regM (reg _ _ a)], M', F') =>
+            Some (ASeq p' (AOp (ROp o (reg' a) x)),
+                [rM a], madd a rM M', F')
+
+        | _ => None
+        end
+
+      | PLet n k m f g =>
+        match (convertProgram' f start M F) with
         | None => None
-        | Some (rp, rr, M', F') =>
-
-          if (list_eq_dec mapping_dec lr rr)
-          then
-            match (G (proj1_sig i0), G (proj1_sig i1)) with
-            | (regM r0, regM r1) => Some (ACond (CReg _ o r0 r1) lp rp, lr, M', F')
-            | (regM r, constM c) => Some (ACond (CConst _ o r c) lp rp, lr, M', F')
-            | _ => None
+        | Some (fp, fm, M', F') =>
+            match (convertProgram' g (start + (length fm)) M' F') with
+            | None => None
+            | Some (gp, gm, M'', F'') => Some (ASeq fp gp, gm, M'', F'')
             end
-          else None
         end
-      end
 
-    | PFunExp n f e => 
-      match (convertProgram' f (S start) M F) with
-      | Some (fp, fr, M', F') => 
-        let a := start in
-        Some (ASeq
-          (AAssign (AConstInt (reg' a) (const' (natToWord _ O))))
-          (AWhile (CConst _ TLt (reg' a) (const' (natToWord _ e)))
-            (ASeq fp (AOp (IOpConst Add (reg' a) (const' (natToWord _ 1)))))),
-          fr, madd a rM M', F')
+      | PComb n a b f g => 
+        match (convertProgram' f start M F) with
+        | None => None
+        | Some (fp, fm, M', F') =>
+            match (convertProgram' g (start + (length fm)) M' F') with
+            | None => None
+            | Some (gp, gm, M'', F'') => Some (ASeq fp gp, fm ++ gm, M'', F'')
+            end
+        end
 
-      | _ => None
-      end
- 
-    | PCall n m lbl f =>
-      match (convertProgram' f start M F) with
-      | Some (fp, fr, M', F') =>
-        let F'' := NatM.add lbl (fp, fr) F' in
-        Some (ACall lbl, fr, M', F'')
-      | None => None
+      | PIf n m o i0 i1 l r => 
+        match (convertProgram' l start M F) with
+        | None => None
+        | Some (lp, lr, lM, lF) =>
+
+            match (convertProgram' r start lM lF) with
+            | None => None
+            | Some (rp, rr, M', F') =>
+
+            if (list_eq_dec mapping_dec lr rr)
+            then
+                match (G (proj1_sig i0), G (proj1_sig i1)) with
+                | (regM r0, regM r1) => Some (ACond (CReg _ o r0 r1) lp rp, lr, M', F')
+                | (regM r, constM c) => Some (ACond (CConst _ o r c) lp rp, lr, M', F')
+                | _ => None
+                end
+            else None
+            end
+        end
+
+      | PFunExp n f e => 
+        match (convertProgram' f (S start) M F) with
+        | Some (fp, fr, M', F') => 
+            let a := start in
+            Some (ASeq
+            (AAssign (AConstInt (reg' a) (const' (natToWord _ O))))
+            (AWhile (CConst _ TLt (reg' a) (const' (natToWord _ e)))
+                (ASeq fp (AOp (IOpConst Add (reg' a) (const' (natToWord _ 1)))))),
+            fr, madd a rM M', F')
+
+        | _ => None
+        end
+
+      | PCall n m lbl f =>
+        match (convertProgram' f start M F) with
+        | Some (fp, fr, M', F') =>
+            let F'' := NatM.add lbl (fp, fr) F' in
+            Some (ACall lbl, fr, M', F'')
+        | None => None
       end
     end.
 
-  Definition convertProgram (prog: Pseudo inVars outVars): option AlmostProgram := 
-    match (convertProgram' prog (max inVars outVars) mempty fempty) with
+  End Conv.
+
+  Definition convertProgram x y (prog: Program x) : option (AlmostQhasm.Program y) := 
+    let vs := max (inputs x) (outputs x) in
+    let M0 := mempty (width x) in
+    let F0 := fempty (width x) in
+
+    match (convertProgram' (width x) (spec x) prog vs M0 F0) with
     | Some (prog', _, M, F) =>
       Some (fold_left
            (fun p0 t => match t with | (k, (v, _)) => ADef k v p0 end)
@@ -188,15 +205,15 @@ Module PseudoConversion <: Conversion Pseudo AlmostQhasm.
     | _ => None
     end.
 
-  Fixpoint convertState (st: AlmostQhasm.State): option State :=
-    let vars := max inVars outVars in
+  Fixpoint convertState x y (st: AlmostQhasm.State y) : option (State x) :=
+    let vars := max (inputs x) (outputs x) in
 
     let try_cons := fun {T} (x: option T) (l: list T) =>
       match x with | Some x' => x' :: l | _ => l end in
 
     let get := fun i =>
-      match (FullState.getReg (reg width_spec i) st,
-             FullState.getStack (stack width_spec i) st) with
+      match (FullState.getReg (reg (spec x) i) st,
+             FullState.getStack (stack (spec x) i) st) with
       | (Some v, _) => Some v
       | (_, Some v) => Some v
       | _ => None
@@ -212,9 +229,10 @@ Module PseudoConversion <: Conversion Pseudo AlmostQhasm.
       else None
     end.
 
-  Lemma convert_spec:  forall a a' b b' prog prog',
-    convertProgram prog = Some prog' ->
-    convertState a = Some a' -> convertState b = Some b' ->
-    AlmostQhasm.evaluatesTo prog' a b <-> evaluatesTo prog a' b'.
+  Lemma convert_spec: forall pa pb a a' b b' prog prog',
+    convertProgram pa pb prog = Some prog' ->
+    convertState pa pb a = Some a' ->
+    convertState pa pb b = Some b' ->
+    AlmostQhasm.evaluatesTo pb prog' a b <-> evaluatesTo pa prog a' b'.
   Admitted.
 End PseudoConversion.
